slsls: some style improvements

theories/simulation/slsls.v
@@ -1,69 +1,73 @@
 (** * SLSLS, Separation Logic Stuttering Local Simulation *)
 
-From iris Require Import bi.bi bi.lib.fixpoint.
-Import bi.
+From iris.bi Require Import bi lib.fixpoint.
 From iris.proofmode Require Import tactics.
 From simuliris.simulation Require Import relations language.
+From iris.prelude Require Import options.
+Import bi.
 
-Class simul_lang (PROP : bi) (Λ : language) := {
+Class SimulLang (PROP : bi) (Λ : language) := {
   (* state interpretation *)
   state_interp : prog Λ → state Λ → prog Λ → state Λ → PROP;
   (* value relation that restricts values passed to functions *)
   val_rel : val Λ → val Λ → PROP;
 }.
 #[global]
-Hint Mode simul_lang + - : typeclass_instances.
+Hint Mode SimulLang + - : typeclass_instances.
 
-Definition progs_are {Λ PROP} `{simul_lang PROP Λ} (P_t P_s: prog Λ) : PROP :=
+Definition progs_are {Λ PROP} `{SimulLang PROP Λ} (P_t P_s : prog Λ) : PROP :=
   (□ ∀ P_t' P_s' σ_t σ_s, state_interp P_t' σ_t P_s' σ_s → ⌜P_t' = P_t⌝ ∧ ⌜P_s' = P_s⌝)%I.
 #[global]
 Hint Mode progs_are - - - + + : typeclass_instances.
 Typeclasses Opaque progs_are.
 
-Global Instance progs_are_persistent {Λ} {PROP} `{s: simul_lang PROP Λ} (P_s P_t: prog Λ): Persistent (@progs_are Λ PROP s P_s P_t).
+Global Instance progs_are_persistent {Λ} {PROP} `{s : SimulLang PROP Λ}
+    (P_s P_t : prog Λ) :
+  Persistent (@progs_are Λ PROP s P_s P_t).
 Proof. rewrite /progs_are; apply _. Qed.
 
 (** Typeclass for the simulation relation so we can use the definitions with
    greatest+least fp (stuttering) or just greatest fp (no stuttering). *)
 (* TODO: remove this TC once we don't need the no-stutter version anymore*)
-Class Sim {PROP : bi} {Λ : language} (s : simul_lang PROP Λ) := sim : expr Λ → expr Λ → (val Λ → val Λ → PROP) → PROP.
+Class Sim {PROP : bi} {Λ : language} (s : SimulLang PROP Λ) :=
+  sim : expr Λ → expr Λ → (val Λ → val Λ → PROP) → PROP.
 #[global]
 Hint Mode Sim - - - : typeclass_instances.
 
-(* FIXME: the notation with binders somehow does not work *)
-(*Notation "et '⪯' es {{ v_t v_s , P }}" := (sim et es (λ v_t v_s, P)) (at level 40, v_t pattern, v_s pattern) : bi_scope.*)
-Notation "et '⪯' es {{ Φ }}" := (sim et es Φ) (at level 40) : bi_scope.
+(* FIXME what are good levels for et, es? *)
+Notation "et  '⪯'  es  {{  Φ  }}" := (sim et es Φ) (at level 40, Φ at level 200) : bi_scope.
+(* FIXME: the notation with binder doesn't work; left-factoring seems to fail.
+Notation "et  '⪯'  es  {{  v_t  v_s ,  P  }}" := (sim et es (λ v_t v_s, P)) (at level 40, v_t, v_s at level 200, P at level 200) : bi_scope. *)
 
 (* discrete OFE instance for expr *)
 Definition exprO {Λ : language} := leibnizO (expr Λ).
 Instance expr_equiv {Λ} : Equiv (expr Λ). apply exprO. Defined.
 
 Section fix_lang.
-  Context {PROP : bi}.
-
+  Context {PROP : bi} `{!BiBUpd PROP, !BiAffine PROP, !BiPureForall PROP}.
   Context {Λ : language}.
-  Context {s : simul_lang PROP Λ}.
+  Context {s : SimulLang PROP Λ}.
 
-  Definition sim_ectx {sim : Sim s} K_t K_s Φ :=
-    (∀ v_t v_s, val_rel v_t v_s -∗ sim (fill K_t (of_val v_t)) (fill K_s (of_val v_s)) Φ)%I.
+  Set Default Proof Using "Type*".
 
   Implicit Types
-    (e_s e_t e: exprO (Λ := Λ))
+    (e_s e_t e: expr Λ)
     (P_s P_t P: prog Λ)
-    (σ_s σ_t σ : state Λ).
+    (σ_s σ_t σ : state Λ)
+    (Φ Ψ : val Λ → val Λ → PROP).
 
-
-  Context {PROP_bupd : BiBUpd PROP}.
-  Context {PROP_affine : BiAffine PROP}.
-  Context {PROP_forall : BiPureForall PROP}.
+  Definition sim_ectx `{!Sim s} K_t K_s Φ :=
+    (∀ v_t v_s, val_rel v_t v_s -∗ sim (fill K_t (of_val v_t)) (fill K_s (of_val v_s)) Φ)%I.
 
   Section stuttering.
     (** Simulation relation with stuttering *)
 
-    Definition least_step (Φ : val Λ → val Λ → PROP) (greatest_rec : exprO → exprO → PROP) (e_s : exprO) (least_rec : exprO → PROP) (e_t : exprO) :=
+    Definition least_step Φ (greatest_rec : exprO → exprO → PROP) e_s
+        (least_rec : exprO → PROP) e_t :=
       (∀ P_t σ_t P_s σ_s, state_interp P_t σ_t P_s σ_s ∗ ⌜¬ reach_stuck P_s e_s σ_s⌝ -∗ |==>
         (* value case *)
-        (∃ v_t v_s σ_s', ⌜to_val e_t = Some v_t⌝ ∗ ⌜rtc (prim_step P_s) (e_s, σ_s) (of_val v_s, σ_s')⌝ ∗
+        (∃ v_t v_s σ_s', ⌜to_val e_t = Some v_t⌝ ∗
+          ⌜rtc (prim_step P_s) (e_s, σ_s) (of_val v_s, σ_s')⌝ ∗
           state_interp P_t σ_t P_s σ_s' ∗ Φ v_t v_s)
 
         ∨ (* step case *)
@@ -71,7 +75,8 @@ Section fix_lang.
           (* stuttering *)
           (state_interp P_t σ_t' P_s σ_s ∗ least_rec e_t') ∨
           (* take a step *)
-          (∃ e_s' σ_s', ⌜tc (prim_step P_s) (e_s, σ_s) (e_s', σ_s')⌝ ∗ state_interp P_t σ_t' P_s σ_s' ∗ greatest_rec e_s' e_t'))
+          (∃ e_s' σ_s', ⌜tc (prim_step P_s) (e_s, σ_s) (e_s', σ_s')⌝ ∗
+            state_interp P_t σ_t' P_s σ_s' ∗ greatest_rec e_s' e_t'))
 
         ∨ (* call case *)
         (∃ f K_t v_t K_s v_s σ_s', ⌜e_t = fill K_t (of_call f v_t)⌝ ∗
@@ -81,8 +86,8 @@ Section fix_lang.
       )%I.
 
     Lemma least_step_mon Φ l1 l2 g1 g2 e_s:
-      ⊢ <pers> (∀ e, l1 e -∗ l2 e)
-      → <pers> (∀ e_s e_t, g1 e_s e_t -∗ g2 e_s e_t)
+      ⊢ □ (∀ e, l1 e -∗ l2 e)
+      → □ (∀ e_s e_t, g1 e_s e_t -∗ g2 e_s e_t)
       → ∀ e, least_step Φ g1 e_s l1 e -∗ least_step Φ g2 e_s l2 e.
     Proof.
       iIntros "#H #H0" (e) "Hl". rewrite /least_step. iIntros (P_t σ_t P_s σ_s) "Ha".
@@ -98,32 +103,35 @@ Section fix_lang.
         iIntros (? ?) "H1". iApply "H0". by iApply "H5".
     Qed.
 
-    Instance least_step_mono (Φ : val Λ → val Λ → PROP) (greatest_rec : exprO → exprO → PROP) (e_s : exprO) :
+    Instance least_step_mono Φ greatest_rec e_s :
       BiMonoPred (least_step Φ greatest_rec e_s).
     Proof.
       constructor.
-      - intros l1 l2. iIntros "H". iApply (least_step_mon Φ l1 l2 greatest_rec greatest_rec e_s with "H").
+      - intros l1 l2. iIntros "H".
+        iApply (least_step_mon Φ l1 l2 greatest_rec greatest_rec e_s with "H").
         eauto.
       - intros l Hne n e1 e2 Heq.
-        apply discrete_iff in Heq as ->. reflexivity. apply _.
+        apply (discrete_iff _ _) in Heq as ->. done.
     Qed.
 
-    Definition least_def (Φ : val Λ → val Λ → PROP) (greatest_rec : exprO → exprO → PROP) (e_s : exprO) :=
+    Definition least_def Φ (greatest_rec : exprO → exprO → PROP) e_s :=
       bi_least_fixpoint (least_step Φ greatest_rec e_s).
 
-    Lemma least_def_unfold (Φ : val Λ → val Λ → PROP) (greatest_rec : exprO → exprO → PROP) (e_s : exprO) e_t:
-      least_def Φ greatest_rec e_s e_t ⊣⊢ least_step Φ greatest_rec e_s (least_def Φ greatest_rec e_s) e_t.
+    Lemma least_def_unfold Φ greatest_rec e_s e_t :
+      least_def Φ greatest_rec e_s e_t ⊣⊢
+        least_step Φ greatest_rec e_s (least_def Φ greatest_rec e_s) e_t.
     Proof. by rewrite /least_def least_fixpoint_unfold. Qed.
 
-    Definition greatest_step (Φ : val Λ → val Λ → PROP) (greatest_rec : exprO * exprO → PROP) '(e_s, e_t) :=
+    Definition greatest_step Φ greatest_rec '(e_s, e_t) :=
       least_def Φ (uncurry greatest_rec) e_s e_t.
 
-    Instance greatest_step_proper Φ greatest_rec:
+    Instance greatest_step_proper Φ greatest_rec :
       Proper ((≡) ==> (≡)) (greatest_step Φ greatest_rec).
     Proof. solve_proper. Qed.
 
     Lemma least_def_mon Φ g1 g2 e_s:
-      ⊢ <pers> (∀ p, g1 p -∗ g2 p) → ∀ e, least_def Φ (uncurry g1) e_s e -∗ least_def Φ (uncurry g2) e_s e.
+      □ (∀ p, g1 p -∗ g2 p) -∗
+      ∀ e, least_def Φ (uncurry g1) e_s e -∗ least_def Φ (uncurry g2) e_s e.
     Proof.
       iIntros "#H".
       rewrite /least_def.
@@ -135,17 +143,17 @@ Section fix_lang.
       - iApply "H0".
     Qed.
 
-    Instance greatest_step_mono (Φ : val Λ → val Λ → PROP) :
+    Instance greatest_step_mono Φ :
       BiMonoPred (greatest_step Φ).
     Proof.
       constructor.
     - intros g1 g2.
       iIntros "#H" ([e_s e_t]) "Hg". rewrite /greatest_step. iApply least_def_mon; eauto.
-    - intros g Hne n [e_s e_t] [e_s' e_t'] Heq. apply discrete_iff in Heq as [-> ->].
-      reflexivity. apply _.
+    - intros g Hne n [e_s e_t] [e_s' e_t'] Heq.
+      apply (discrete_iff _ _) in Heq as [-> ->]. done.
     Qed.
 
-    Definition sim_def (Φ : val Λ → val Λ → PROP) :=
+    Definition sim_def Φ :=
       bi_greatest_fixpoint (greatest_step Φ).
 
     Lemma sim_def_unfold Φ e_s e_t:
@@ -156,9 +164,12 @@ Section fix_lang.
       sim_def Φ (e_s, e_t) ⊣⊢ least_def Φ (uncurry (sim_def Φ)) e_s e_t.
     Proof. by rewrite sim_def_unfold. Qed.
 
-    Definition sim_aux : seal (λ e_t e_s Φ, @sim_def Φ (e_s, e_t)). by eexists. Qed.
-    Instance sim_stutter : Sim s. exact ((sim_aux).(unseal)). Defined.
-    Definition sim_eq : sim_stutter = λ e_t e_s Φ, @sim_def Φ (e_s, e_t). by rewrite <- (sim_aux).(seal_eq). Defined.
+    Definition sim_aux : seal (λ e_t e_s Φ, @sim_def Φ (e_s, e_t)).
+    Proof. by eexists. Qed.
+    (* Instance is local to avoid ambiguity. *)
+    Instance sim_stutter : Sim s := sim_aux.(unseal).
+    Lemma sim_eq : sim (Sim:=sim_stutter) = λ e_t e_s Φ, @sim_def Φ (e_s, e_t).
+    Proof. rewrite -sim_aux.(seal_eq) //. Qed.
 
     Lemma sim_unfold Φ e_t e_s:
       sim (Sim:=sim_stutter) e_t e_s Φ ⊣⊢
@@ -169,44 +180,45 @@ Section fix_lang.
 
         ∨ (* step case *)
         (⌜reducible P_t e_t σ_t⌝ ∗ ∀ e_t' σ_t', ⌜prim_step P_t (e_t, σ_t) (e_t', σ_t')⌝ -∗ |==>
-          (state_interp P_t σ_t' P_s σ_s ∗ sim (Sim:=sim_stutter) e_t' e_s Φ) ∨
+          (state_interp P_t σ_t' P_s σ_s ∗ sim e_t' e_s Φ) ∨
           (∃ e_s' σ_s', ⌜tc (prim_step P_s) (e_s, σ_s) (e_s', σ_s')⌝ ∗ state_interp P_t σ_t' P_s σ_s' ∗
-          sim (Sim:=sim_stutter) e_t' e_s' Φ))
+          sim e_t' e_s' Φ))
 
         ∨ (* call case *)
         (∃ f K_t v_t K_s v_s σ_s', ⌜e_t = fill K_t (of_call f v_t)⌝ ∗
           ⌜rtc (prim_step P_s) (e_s, σ_s) (fill K_s (of_call f v_s), σ_s')⌝ ∗
           val_rel v_t v_s ∗ state_interp P_t σ_t P_s σ_s' ∗
-          sim_ectx (sim:=sim_stutter) K_t K_s Φ)
+          sim_ectx K_t K_s Φ)
       )%I.
     Proof.
-      rewrite /sim_ectx /sim !sim_eq /uncurry sim_def_unfold /greatest_step.
+      rewrite /sim_ectx !sim_eq /uncurry sim_def_unfold /greatest_step.
       rewrite least_def_unfold /least_step.
-      by setoid_rewrite <-sim_def_least_def_unfold.
+      setoid_rewrite <-sim_def_least_def_unfold. done.
     Qed.
 
     (* any post-fixed point is included in the gfp *)
-    Lemma sim_coind Φ (Ψ : exprO → exprO → PROP):
+    Lemma sim_coind Φ (Ψ : exprO → exprO → PROP) :
       Proper ((≡) ==> (≡) ==> (≡)) Ψ →
       ⊢ (□ ∀ e_t e_s, Ψ e_t e_s -∗ greatest_step Φ (λ '(e_s, e_t), Ψ e_t e_s) (e_s, e_t))
         -∗ ∀ e_t e_s, Ψ e_t e_s -∗ sim e_t e_s Φ.
     Proof.
       iIntros (Hp) "#H". iIntros (e_t e_s) "H0".
-      rewrite /sim sim_eq /sim_def.
+      rewrite sim_eq /sim_def.
 
       set (Ψ_curry := (λ '(e_t, e_s), Ψ e_s e_t)).
       assert (NonExpansive Ψ_curry) as Hne.
       { intros ? [e1 e2] [e1' e2'] [H1 H2]. rewrite /Ψ_curry. cbn in H1, H2.
-        apply equiv_dist, Hp. now apply discrete_iff in H1. now apply discrete_iff in H2.
+        apply equiv_dist, Hp.
+        - by apply (discrete_iff _ _) in H1.
+        - by apply (discrete_iff _ _) in H2.
       }
       iApply (greatest_fixpoint_coind (greatest_step Φ) Ψ_curry).
       { iModIntro. iIntros ([e_s' e_t']). iApply "H". }
       iApply "H0".
     Qed.
 
-
     (* TODO: not sure yet if this lemma is useful. if not, remove *)
-    Lemma sim_strong_ind' (e_s : exprO) Φ (Ψ : exprO → exprO → (val Λ → val Λ → PROP) → PROP):
+    Lemma sim_strong_ind' e_s Φ (Ψ : exprO → exprO → (val Λ → val Λ → PROP) → PROP):
       Proper ((≡) ==> (≡) ==> (pointwise_relation (val Λ) (pointwise_relation (val Λ) (≡))) ==> (≡)) Ψ →
       ⊢ (□ ∀ e_t, least_step Φ (uncurry (sim_def Φ)) e_s
               (λ e_t', Ψ e_t' e_s Φ ∧ least_def Φ (uncurry (sim_def Φ)) e_s e_t')
@@ -214,7 +226,7 @@ Section fix_lang.
         -∗ ∀ e_t : exprO, (e_t ⪯ e_s {{ Φ }}) -∗ Ψ e_t e_s Φ.
     Proof.
       iIntros (Hp) "#IH". iIntros (e_t).
-      rewrite /sim sim_eq /sim_def.
+      rewrite sim_eq /sim_def.
       rewrite greatest_fixpoint_unfold {2}/greatest_step /least_def.
 
       change (bi_greatest_fixpoint (greatest_step Φ)) with (sim_def Φ).
@@ -228,10 +240,10 @@ Section fix_lang.
     Qed.
 
     (* TODO: not sure yet if this lemma is useful. if not, remove *)
-    Lemma sim_ind' (e_s : exprO) Φ (Ψ : exprO → exprO → (val Λ → val Λ → PROP) → PROP):
+    Lemma sim_ind' e_s Φ (Ψ : exprO → exprO → (val Λ → val Λ → PROP) → PROP):
       Proper ((≡) ==> (≡) ==> (pointwise_relation (val Λ) (pointwise_relation (val Λ) (≡))) ==> (≡)) Ψ →
       ⊢ (□ ∀ e_t, least_step Φ (uncurry (sim_def Φ)) e_s (λ e_t', Ψ e_t' e_s Φ) e_t -∗ Ψ e_t e_s Φ)
-        -∗ ∀ e_t : exprO, e_t ⪯ e_s {{Φ}} -∗ Ψ e_t e_s Φ.
+        -∗ ∀ e_t : exprO, e_t ⪯ e_s {{ Φ }} -∗ Ψ e_t e_s Φ.
     Proof.
       iIntros (Hp) "#IH". iApply sim_strong_ind'. iModIntro.
       iIntros (e_t) "H". iApply "IH".
@@ -239,30 +251,34 @@ Section fix_lang.
       iModIntro. by iIntros (e) "[H _]".
     Qed.
 
-    Lemma sim_strong_ind greatest_rec (e_s : exprO) Φ (Ψ : exprO → PROP):
+    Lemma sim_strong_ind greatest_rec e_s Φ (Ψ : exprO → PROP):
       Proper ((≡) ==> (≡)) Ψ →
-      ⊢ (□ ∀ e_t, least_step Φ greatest_rec e_s
+      (□ ∀ e_t, least_step Φ greatest_rec e_s
             (λ e_t', Ψ e_t' ∧ least_def Φ greatest_rec e_s e_t')
-          e_t -∗ Ψ e_t)
-        -∗ ∀ e_t : exprO, least_def Φ greatest_rec e_s e_t -∗ Ψ e_t.
+        e_t -∗ Ψ e_t) -∗
+      ∀ e_t : exprO, least_def Φ greatest_rec e_s e_t -∗ Ψ e_t.
     Proof.
       iIntros (Hp) "#H". iApply least_fixpoint_strong_ind.
       iModIntro. iIntros (e_t) "IH". by iApply "H".
     Qed.
 
-    Lemma sim_ind greatest_rec (e_s : exprO) Φ (Ψ : exprO → PROP):
+    Lemma sim_ind greatest_rec e_s Φ (Ψ : exprO → PROP):
       Proper ((≡) ==> (≡)) Ψ →
-      ⊢ (□ ∀ e_t, least_step Φ greatest_rec e_s Ψ e_t -∗ Ψ e_t)
-        -∗ ∀ e_t : exprO, least_def Φ greatest_rec e_s e_t -∗ Ψ e_t.
-    Proof. iIntros (Hp) "#H". iApply least_fixpoint_ind. iModIntro. iIntros (e_t) "IH". by iApply "H". Qed.
+      (□ ∀ e_t, least_step Φ greatest_rec e_s Ψ e_t -∗ Ψ e_t) -∗
+      ∀ e_t : exprO, least_def Φ greatest_rec e_s e_t -∗ Ψ e_t.
+    Proof.
+      iIntros (Hp) "#H". iApply least_fixpoint_ind.
+      iIntros "!>" (e_t) "IH". by iApply "H".
+    Qed.
 
     Instance sim_proper :
-      Proper (eq ==> eq ==> (pointwise_relation (val Λ) (pointwise_relation (val Λ) (≡))) ==> (≡)) sim.
+      Proper (eq ==> eq ==>
+        (pointwise_relation (val Λ) (pointwise_relation (val Λ) (≡))) ==> (≡)) sim.
     Proof.
       intros e e' -> e1 e1' -> p1 p2 Heq2.
-      rewrite /sim !sim_eq. apply greatest_fixpoint_proper; last reflexivity.
+      rewrite !sim_eq. apply greatest_fixpoint_proper; last done.
       intros p3 [e3 e3']. rewrite /greatest_step /least_def.
-      apply least_fixpoint_proper; last reflexivity. solve_proper.
+      apply least_fixpoint_proper; last done. solve_proper.
     Qed.
 
     Lemma sim_value_target Φ v_t e_s v_s:
@@ -270,30 +286,31 @@ Section fix_lang.
     Proof.
       iIntros "Hv Hr". rewrite sim_unfold. iIntros (????) "[Hstate Hreach]".
       iModIntro. iLeft. iExists (v_t), (v_s), (σ_s). iFrame.
-      iSplitL "". by rewrite to_of_val. eauto.
+      iSplitR; first by rewrite to_of_val. eauto.
     Qed.
 
     Lemma sim_value Φ v_t v_s:
-      ⊢ (Φ v_t v_s) -∗ (of_val v_t) ⪯ (of_val v_s) {{Φ}}.
+      ⊢ (Φ v_t v_s) -∗ (of_val v_t) ⪯ (of_val v_s) {{ Φ }}.
     Proof.
       iIntros "Hv". rewrite sim_unfold. iIntros (????) "[Hstate Hreach]".
       iModIntro. iLeft. iExists (v_t), (v_s), (σ_s). iFrame.
-      iSplitL. by rewrite to_of_val. eauto.
+      iSplitL; first by rewrite to_of_val. eauto.
     Qed.
 
+    (* FIXME(RJ) this lemma leaks implementation details? *)
     Lemma sim_stutter_incl Φ e_s e_t:
       ⊢ least_def Φ (uncurry (sim_def Φ)) e_s e_t
-        -∗ e_t ⪯ e_s {{Φ}}.
-    Proof. iIntros "H". by rewrite /sim sim_eq sim_def_unfold /greatest_step. Qed.
+        -∗ e_t ⪯ e_s {{ Φ }}.
+    Proof. iIntros "H". by rewrite sim_eq sim_def_unfold /greatest_step. Qed.
 
     Lemma bupd_sim Φ e_t e_s:
-      ⊢ (|==> e_t ⪯ e_s {{Φ}}) -∗ e_t ⪯ e_s {{Φ}}.
+      ⊢ (|==> e_t ⪯ e_s {{ Φ }}) -∗ e_t ⪯ e_s {{ Φ }}.
     Proof.
       iIntros "Hv". rewrite sim_unfold. iIntros (????) "H". iMod "Hv". iApply ("Hv" with "H").
     Qed.
 
     Lemma sim_bupd Φ e_t e_s:
-      ⊢ (e_t ⪯ e_s {{λ v_t v_s, |==> Φ v_t v_s}}) -∗ e_t ⪯ e_s {{Φ}}.
+      ⊢ (e_t ⪯ e_s {{ λ v_t v_s, |==> Φ v_t v_s }}) -∗ e_t ⪯ e_s {{ Φ }}.
     Proof.
       iIntros "Hv".
       iApply (sim_coind Φ (λ e_t e_s, e_t ⪯ e_s {{λ v_t v_s, |==> Φ v_t v_s}})%I); last by iFrame.
@@ -306,7 +323,7 @@ Section fix_lang.
       - iModIntro. iRight; iLeft. iDestruct "H" as "[Hred H]"; iFrame.
         iIntros (??) "Hs". iMod ("H" with "Hs") as "[[? Hs] | Hs]"; iModIntro.
         + iLeft. iFrame.
-          iApply sim_ind. 2: { rewrite /sim sim_eq sim_def_least_def_unfold. iFrame. }
+          iApply sim_ind. 2: { rewrite sim_eq sim_def_least_def_unfold. iFrame. }
           iModIntro. clear e_t' P_t P_s σ_t' σ_t σ_s. iIntros (e_t') "IH".
           rewrite least_def_unfold !/least_step.
           iIntros (????) "H". iMod ("IH" with "H") as "Hv".
@@ -316,47 +333,53 @@ Section fix_lang.
           * iModIntro. iRight; iLeft. iDestruct "H" as "[Hred H]"; iFrame.
             iIntros (??) "Hs". iMod ("H" with "Hs") as "[[? Hs] | Hs]"; iModIntro.
             { iLeft. iFrame. }
-            iRight. rewrite /sim sim_eq. iFrame.
-          * iModIntro. iRight; iRight. rewrite /sim sim_eq. iFrame.
+            iRight. rewrite sim_eq. iFrame.
+          * iModIntro. iRight; iRight. rewrite sim_eq. iFrame.
         + iRight. iFrame.
       - iModIntro. iRight; iRight. iFrame.
     Qed.
 
     (* we change the predicate beause at every recursive ocurrence,
        we give back ownership of the monotonicity assumption *)
-    Lemma least_def_mono rec Φ Φ':
-      ⊢ (∀ v_t v_s, Φ v_t v_s -∗ Φ' v_t v_s)
-        -∗ ∀ e_s e_t : exprO, least_def Φ rec e_s e_t -∗
-        least_def Φ' (λ e_s e_t, rec e_s e_t ∗ ∀ v_t v_s, Φ v_t v_s -∗ Φ' v_t v_s) e_s e_t.
+    Lemma least_def_mono rec Φ Φ' :
+      (∀ v_t v_s, Φ v_t v_s -∗ Φ' v_t v_s) -∗
+      ∀ e_s e_t,
+      least_def Φ rec e_s e_t -∗
+      least_def Φ' (λ e_s e_t, rec e_s e_t ∗ ∀ v_t v_s, Φ v_t v_s -∗ Φ' v_t v_s) e_s e_t.
     Proof.
       iIntros "Hmon" (e_s e_t). iIntros "Hleast". iRevert "Hmon".
       iApply (sim_ind _ _ _ (λ e_t, (∀ v_t v_s : val Λ, Φ v_t v_s -∗ Φ' v_t v_s) -∗ least_def Φ' (λ e_s e_t, rec e_s e_t ∗ ∀ v_t v_s, Φ v_t v_s -∗ Φ' v_t v_s) e_s e_t)%I with "[] Hleast"); clear e_t.
       iModIntro. iIntros (e_t) "IH Hmon". rewrite least_def_unfold /least_step.
       iIntros (P_t σ_t P_s σ_s) "H". iMod ("IH" with "H") as "IH". iModIntro.
       iDestruct "IH" as "[Hval | [Hstep | Hcall]]".
-      - iLeft. iDestruct "Hval" as (v_t v_s σ_s') "(?&?&?&?)". iExists v_t, v_s, σ_s'. iFrame. by iApply "Hmon".
-      - iRight; iLeft. iDestruct "Hstep" as "[$ Hstep]". iIntros (e_t' σ_t' Hstep).
+      - iLeft. iDestruct "Hval" as (v_t v_s σ_s') "(?&?&?&?)".
+        iExists v_t, v_s, σ_s'. iFrame. by iApply "Hmon".
+      - iRight; iLeft. iDestruct "Hstep" as "[$ Hstep]".
+        iIntros (e_t' σ_t' Hstep).
         iMod ("Hstep" with "[//]") as "[Hstep|Hstep]".
         + iModIntro. iLeft. iDestruct "Hstep" as "[$ H]". by iApply "H".
         + iModIntro. iRight. iFrame "Hmon". eauto.
       - iRight; iRight. by iFrame "Hmon".
     Qed.
 
-    Lemma sim_mono Φ Φ':
-      ⊢ (∀ v_t v_s, Φ v_t v_s -∗ Φ' v_t v_s)
-         -∗ ∀ e_s e_t : exprO, e_t ⪯ e_s {{Φ}} -∗ e_t ⪯ e_s {{Φ'}}.
+    Lemma sim_mono Φ Φ' :
+      (∀ v_t v_s, Φ v_t v_s -∗ Φ' v_t v_s) -∗
+      ∀ e_s e_t : exprO, e_t ⪯ e_s {{ Φ }} -∗ e_t ⪯ e_s {{ Φ' }}.
     Proof.
       iIntros "Hmon" (e_s e_t) "H".
-      iApply (sim_coind Φ' (λ e_t e_s, e_t ⪯ e_s {{Φ}} ∗ (∀ v_t v_s : val Λ, Φ v_t v_s -∗ Φ' v_t v_s))%I); last by iFrame.
+      iApply (sim_coind Φ' (λ e_t e_s, e_t ⪯ e_s {{ Φ }} ∗ (∀ v_t v_s : val Λ, Φ v_t v_s -∗ Φ' v_t v_s))%I); last by iFrame.
       iModIntro. clear e_t e_s. iIntros (e_t e_s) "[H Hmon]".
-      rewrite /sim sim_eq sim_def_unfold.
+      rewrite sim_eq sim_def_unfold.
       rewrite /greatest_step !least_def_unfold /least_step.
       iIntros (????) "Hs". iSpecialize ("H" with "Hs"). iMod "H". iModIntro.
       iDestruct "H" as "[Hval | [Hred | Hcall]]".
-      - iLeft. iDestruct "Hval" as (v_t v_s σ_s') "(?&?&?&?)". iExists v_t, v_s, σ_s'. iFrame. by iApply "Hmon".
+      - iLeft. iDestruct "Hval" as (v_t v_s σ_s') "(?&?&?&?)".
+        iExists v_t, v_s, σ_s'. iFrame. by iApply "Hmon".
       - iRight; iLeft. iDestruct "Hred" as "[Hred Hstep]". iFrame.
-        iIntros (e_t' σ_t') "Hprim". iMod ("Hstep" with "Hprim") as "[Hstutter | Hstep]"; iModIntro.
-        + iLeft. iDestruct "Hstutter" as "[Hstate Hleast]". iFrame. by iApply (least_def_mono with "Hmon").
+        iIntros (e_t' σ_t') "Hprim".
+        iMod ("Hstep" with "Hprim") as "[Hstutter | Hstep]"; iModIntro.
+        + iLeft. iDestruct "Hstutter" as "[Hstate Hleast]". iFrame.
+          by iApply (least_def_mono with "Hmon").
         + iRight. by iFrame.
       - iRight; iRight. iFrame.
     Qed.
@@ -365,7 +388,7 @@ Section fix_lang.
     (* coinduction predicate used for the bind lemma *)
     Definition bind_pred Φ := uncurry (λ '(e_s, e_t), ∃ e_t' e_s' (K_t K_s : ectx Λ),
       ⌜e_t = fill K_t e_t'⌝ ∧ ⌜e_s = fill K_s e_s'⌝ ∧
-       e_t' ⪯ e_s' {{λ v_t v_s : val Λ, fill K_t (of_val v_t) ⪯ fill K_s (of_val v_s) {{Φ}}}})%I.
+       e_t' ⪯ e_s' {{ λ v_t v_s : val Λ, fill K_t (of_val v_t) ⪯ fill K_s (of_val v_s) {{ Φ }} }})%I.
 
     (* Lemma used two times in the proof of the bind lemma (for the value cases of the inner and outer induction) *)
     Lemma sim_bind_val P_s e_s σ_s v_s σ_s' e_t v_t K_t σ_t P_t K_s Φ:
@@ -400,11 +423,11 @@ Section fix_lang.
     Proof.
       (* unfold Hpost to examine the result and combine the two simulation proofs *)
       iIntros (H0 H Hnreach) "Hpost Hstate".
-      rewrite {1}/sim {1}sim_eq {1}sim_def_unfold.
+      rewrite {1}sim_eq {1}sim_def_unfold.
       rewrite {1}/greatest_step !least_def_unfold /least_step.
       iMod ("Hpost" with "[Hstate]") as "Hpost".
       { iFrame. iPureIntro. intros Hstuck. eapply Hnreach, prim_step_rtc_reach_stuck.
-        by apply fill_prim_step_rtc. assumption. }
+        1:by apply fill_prim_step_rtc. assumption. }
       iModIntro.
       iDestruct "Hpost" as "[Hv | [Hstep | Hcall]]".
       + iLeft. iDestruct "Hv" as (v_t' v_s' σ_s'') "(% & % & Hstate & Hpost)".
@@ -421,8 +444,8 @@ Section fix_lang.
           { injection Heq as ??; subst. iLeft. iFrame. iApply least_def_mon. 2: iApply "Hstutter".
             iModIntro. iIntros ([e_s e_t'']) "H".
             iExists e_t'', e_s, empty_ectx, empty_ectx.
-            rewrite !fill_empty. do 2 (iSplitL ""; first auto).
-            iApply sim_mono. 2: { rewrite /sim sim_eq. iApply "H". }
+            rewrite !fill_empty. do 2 (iSplitR; first auto).
+            iApply sim_mono. 2: { rewrite sim_eq. iApply "H". }
             iIntros (v_t' v_s') "Hv". rewrite !fill_empty. by iApply sim_value.
           }
           {
@@ -430,29 +453,29 @@ Section fix_lang.
             iSplitR "Hstutter".
             { iPureIntro. by apply fill_prim_step_tc. }
             cbn. iExists e_t', (fill K_s (of_val v_s)), empty_ectx, empty_ectx. rewrite !fill_empty.
-            do 2 (iSplitL ""; first auto).
+            do 2 (iSplitR; first auto).
             iApply sim_mono. 2: { iApply sim_stutter_incl. iApply "Hstutter". }
             iIntros (v_t' v_s') "Hv". rewrite !fill_empty. by iApply sim_value.
           }
         * iDestruct "Hstep" as (e_s' σ_s'') "(%&Hstate& Hrec)". iRight.
-          iExists e_s', σ_s''. iFrame. iSplitL "".
+          iExists e_s', σ_s''. iFrame. iSplitR.
           { iPureIntro. eapply tc_rtc_l; by eauto using fill_prim_step_rtc. }
           cbn. iExists e_t', e_s', empty_ectx, empty_ectx. rewrite !fill_empty.
-          do 2 (iSplitL ""; first auto).
-          iApply sim_mono. 2: { rewrite /sim sim_eq. iApply "Hrec". }
+          do 2 (iSplitR; first auto).
+          iApply sim_mono. 2: { rewrite sim_eq. iApply "Hrec". }
           iIntros (??) "H". rewrite !fill_empty.
           by iApply sim_value.
       + iDestruct "Hcall" as (f K_t' v_t' K_s' v_s' σ_s'') "(%&%&Hvrel&Hstate&Hcall)".
         (* CA on the reduction of fill K_s v_s to fill K_s' (f v_s') to see if we need to take a step or do the call *)
         iRight; iRight.
         iExists f, K_t', v_t', K_s', v_s', σ_s''. iFrame.
-        iSplitL "". { iPureIntro. by rewrite -H1 (of_to_val _ _ H). }
-        iSplitL "". { iPureIntro. etrans; eauto using fill_prim_step_rtc. }
+        iSplitR. { iPureIntro. by rewrite -H1 (of_to_val _ _ H). }
+        iSplitR. { iPureIntro. etrans; eauto using fill_prim_step_rtc. }
         iIntros (v_t'' v_s'') "Hvrel". cbn.
         iExists (fill K_t' (of_val v_t'')), (fill K_s' (of_val v_s'')), empty_ectx, empty_ectx.
-        rewrite !fill_empty. do 2 (iSplitL ""; first auto).
+        rewrite !fill_empty. do 2 (iSplitR; first auto).
         iApply sim_mono; first last.
-        { rewrite /sim sim_eq. by iApply "Hcall". }
+        { rewrite sim_eq. by iApply "Hcall". }
         iIntros (??) "H". rewrite !fill_empty. by iApply sim_value.
     Qed.
 
@@ -466,7 +489,7 @@ Section fix_lang.
       iModIntro. clear e_t e_s K_t K_s.
       iIntros (e_t' e_s') "IH".
       iDestruct "IH" as (e_t e_s K_t K_s) "[-> [-> H]]".
-      rewrite {1}/sim {1}sim_eq {1}sim_def_unfold.
+      rewrite {1}sim_eq {1}sim_def_unfold.
       rewrite /greatest_step !least_def_unfold /least_step.
 
       iIntros (????) "[Hs %]". rename H into Hnreach.
@@ -477,7 +500,7 @@ Section fix_lang.
         by iApply (sim_bind_val with "[Hpost] [Hstate]").
       - (* simply thread through everything *)
         iModIntro. iRight; iLeft. iDestruct "Hstep" as "[% Hstep]".
-        iSplitL "". { iPureIntro. by apply fill_reducible. }
+        iSplitR. { iPureIntro. by apply fill_reducible. }
         iIntros (e_t' σ_t') "%".
         destruct (fill_reducible_prim_step _ _ _ _ _ _ H H0) as (e_t'' & -> & H1).
         iMod ("Hstep" with "[]") as "Hstep". { iPureIntro. apply H1. }
@@ -492,42 +515,41 @@ Section fix_lang.
           iDestruct "IH" as "[Hval | [Hred | Hcall]]".
           * iDestruct "Hval" as (v_t v_s σ_s') "(% & % & Hstate & Hrec)".
             by iApply (sim_bind_val with "[Hrec] [Hstate]").
-          * iModIntro. iDestruct "Hred" as "[% Hred]". iRight; iLeft. iSplitL "".
+          * iModIntro. iDestruct "Hred" as "[% Hred]". iRight; iLeft. iSplitR.
             { iPureIntro. by apply fill_reducible. }
             iIntros (e_t' σ_t'') "%".
             destruct (fill_reducible_prim_step _ _ _ _ _ _ H0 H1) as (e_t''' & -> & H2).
-            iMod ("Hred" with "[ //]") as "[Hstutter | Hstep]"; iModIntro.
-            by iLeft.
+            iMod ("Hred" with "[ //]") as "[Hstutter | Hstep]"; iModIntro; first by iLeft.
             iRight. iDestruct "Hstep" as (e_s' σ_s') "(%&Hstate&Hrec)".
-            iExists (fill K_s e_s'), σ_s'. iFrame. iSplitL "".
+            iExists (fill K_s e_s'), σ_s'. iFrame. iSplitR.
             { iPureIntro. by apply fill_prim_step_tc. }
-            cbn. iExists e_t''', e_s', K_t, K_s. do 2 (iSplitL ""; first auto).
-            by rewrite /sim sim_eq.
+            cbn. iExists e_t''', e_s', K_t, K_s. do 2 (iSplitR; first auto).
+            by rewrite sim_eq.
           * iModIntro. iDestruct "Hcall" as (f K_t' v_t K_s' v_s σ_s') "(-> & % & Hv & Hstate & Hcall)".
             iRight; iRight. iExists f, (comp_ectx K_t K_t'), v_t, (comp_ectx K_s K_s'), v_s, σ_s'.
-            iSplitL "". { by rewrite fill_comp. }
-            iSplitL "". { iPureIntro. rewrite -fill_comp. by apply fill_prim_step_rtc. }
+            iSplitR. { by rewrite fill_comp. }
+            iSplitR. { iPureIntro. rewrite -fill_comp. by apply fill_prim_step_rtc. }
             iFrame. iIntros (v_t' v_s') "Hv".
             cbn. iExists (fill K_t' (of_val v_t')), (fill K_s' (of_val v_s')), K_t, K_s.
-            rewrite !fill_comp. do 2 (iSplitL ""; first auto).
-            rewrite /sim sim_eq. by iApply "Hcall".
+            rewrite !fill_comp. do 2 (iSplitR; first auto).
+            rewrite sim_eq. by iApply "Hcall".
         + iRight. iDestruct "Hstep" as (e_s' σ_s') "(% & Hstate & Hrec)".
-          iExists (fill K_s e_s'), σ_s'. iFrame. iSplitL "".
+          iExists (fill K_s e_s'), σ_s'. iFrame. iSplitR.
           { iPureIntro. by apply fill_prim_step_tc. }
           cbn. iExists e_t'', e_s', K_t, K_s.
-          do 2 (iSplitL ""; first auto).
-          rewrite /sim sim_eq. iApply "Hrec".
+          do 2 (iSplitR; first auto).
+          rewrite sim_eq. iApply "Hrec".
       - (* simply thread through everything *)
         iModIntro. iRight; iRight.
         iDestruct "Hcall" as (f K_t' v_t K_s' v_s σ_s') "(-> & % & Hval & Hstate & Hrec)".
         iExists f, (comp_ectx K_t K_t'), v_t, (comp_ectx K_s K_s'), v_s, σ_s'.
-        iSplitL "". by rewrite fill_comp.
-        iSplitL "". { iPureIntro. rewrite -fill_comp. by apply fill_prim_step_rtc. }
+        iSplitR; first by rewrite fill_comp.
+        iSplitR. { iPureIntro. rewrite -fill_comp. by apply fill_prim_step_rtc. }
         iFrame.
         iIntros (v_t' v_s') "Hv". iSpecialize ("Hrec" with "Hv"). cbn.
         iExists (fill K_t' (of_val v_t')), (fill K_s' (of_val v_s')), K_t, K_s.
-        iSplitL "". by rewrite -fill_comp. iSplitL "". by rewrite -fill_comp.
-        rewrite /sim sim_eq. iApply "Hrec".
+        iSplitR; first by rewrite -fill_comp. iSplitR; first by rewrite -fill_comp.
+        rewrite sim_eq. iApply "Hrec".
     Qed.
 
 
@@ -553,47 +575,52 @@ Section fix_lang.
     Qed.
 
     Lemma sim_frame_r e_t e_s R Φ :
-      e_t ⪯ e_s {{Φ}} ∗ R ⊢ e_t ⪯ e_s {{λ v_t v_s, Φ v_t v_s ∗ R}}.
+      e_t ⪯ e_s {{ Φ }} ∗ R ⊢ e_t ⪯ e_s {{λ v_t v_s, Φ v_t v_s ∗ R}}.
     Proof.
       iIntros "[Hsim HR]". iApply (sim_mono with "[HR] [Hsim//]"). iIntros (v_t v_s) "H". iFrame.
     Qed.
 
     Lemma sim_frame_l e_t e_s R Φ :
-      R ∗ e_t ⪯ e_s {{Φ}} ⊢ e_t ⪯ e_s {{λ v_t v_s, R ∗ Φ v_t v_s}}.
+      R ∗ e_t ⪯ e_s {{ Φ }} ⊢ e_t ⪯ e_s {{λ v_t v_s, R ∗ Φ v_t v_s}}.
     Proof.
       iIntros "[HR Hsim]". iApply (sim_mono with "[HR] [Hsim//]"). iIntros (v_t v_s) "H". iFrame.
     Qed.
 
-    Lemma sim_wand e_t e_s Φ Ψ:
-      e_t ⪯ e_s {{Φ}} -∗ (∀ v_t v_s, Φ v_t v_s -∗ Ψ v_t v_s) -∗ e_t ⪯ e_s {{Ψ}}.
+    Lemma sim_wand e_t e_s Φ Ψ :
+      e_t ⪯ e_s {{ Φ }} -∗ (∀ v_t v_s, Φ v_t v_s -∗ Ψ v_t v_s) -∗ e_t ⪯ e_s {{ Ψ }}.
     Proof. iIntros "H Hv". iApply (sim_mono with "[Hv//] [H//]"). Qed.
 
-    Lemma sim_wand_l e_t e_s Φ Ψ:
-      (∀ v_t v_s, Φ v_t v_s -∗ Ψ v_t v_s) ∗ e_t ⪯ e_s {{Φ}} ⊢ e_t ⪯ e_s {{Ψ}}.
+    Lemma sim_wand_l e_t e_s Φ Ψ :
+      (∀ v_t v_s, Φ v_t v_s -∗ Ψ v_t v_s) ∗ e_t ⪯ e_s {{ Φ }} ⊢ e_t ⪯ e_s {{ Ψ }}.
     Proof. iIntros "[Hv H]". iApply (sim_wand with "[H//] [Hv//]"). Qed.
 
-    Lemma sim_wand_r e_t e_s Φ Ψ:
-      e_t ⪯ e_s {{Φ}} ∗ (∀ v_t v_s, Φ v_t v_s -∗ Ψ v_t v_s) ⊢ e_t ⪯ e_s {{Ψ}}.
+    Lemma sim_wand_r e_t e_s Φ Ψ :
+      e_t ⪯ e_s {{ Φ }} ∗ (∀ v_t v_s, Φ v_t v_s -∗ Ψ v_t v_s) ⊢ e_t ⪯ e_s {{ Ψ }}.
     Proof. iIntros "[H Hv]". iApply (sim_wand with "[H//] [Hv//]"). Qed.
 
-    Lemma sim_stutter_source e_t e_s Φ:
-      ⊢ (∀ P_t P_s σ_t σ_s, state_interp P_t σ_t P_s σ_s ==∗ ⌜reducible P_t e_t σ_t⌝ ∗ ∀ e_t' σ_t',
-          ⌜ prim_step P_t (e_t, σ_t) (e_t', σ_t') ⌝ ==∗ state_interp P_t σ_t' P_s σ_s ∗ e_t' ⪯ e_s {{ Φ }}) -∗
+    Lemma sim_stutter_source e_t e_s Φ :
+      ⊢ (∀ P_t P_s σ_t σ_s, state_interp P_t σ_t P_s σ_s ==∗
+          ⌜reducible P_t e_t σ_t⌝ ∗
+          ∀ e_t' σ_t', ⌜prim_step P_t (e_t, σ_t) (e_t', σ_t')⌝ ==∗
+            state_interp P_t σ_t' P_s σ_s ∗ e_t' ⪯ e_s {{ Φ }}) -∗
         e_t ⪯ e_s {{ Φ }}.
     Proof.
       iIntros "H". rewrite (sim_unfold Φ e_t e_s). iIntros (????) "[H1 H2]".
       iMod ("H" with "H1") as "H". iModIntro. iRight; iLeft. iDestruct "H" as "(% & Hnext)".
-      iSplitL "". { by iPureIntro. }
+      iSplitR. { by iPureIntro. }
       iIntros (e_t' σ_t') "Hstep". iMod ("Hnext" with "Hstep") as "[Hstate Hsim]".
       iModIntro. iLeft. iFrame.
     Qed.
 
     (* the step case of the simulation relation, but the two cases are combined into an rtc in the source *)
     Lemma sim_step_target e_t e_s Φ:
-      ⊢ ( ∀ P_t P_s σ_t σ_s, state_interp P_t σ_t P_s σ_s ==∗ ⌜ reducible P_t e_t σ_t⌝ ∗ (∀ e_t' σ_t',
-          ⌜ prim_step P_t (e_t, σ_t) (e_t', σ_t') ⌝ ==∗ ∃ e_s' σ_s',
-          ⌜ rtc (prim_step P_s) (e_s, σ_s) (e_s', σ_s') ⌝ ∗ state_interp P_t σ_t' P_s σ_s' ∗ e_t' ⪯ e_s' {{Φ}})) -∗
-        e_t ⪯ e_s {{Φ}}.
+      (∀ P_t P_s σ_t σ_s, state_interp P_t σ_t P_s σ_s ==∗
+        ⌜reducible P_t e_t σ_t⌝ ∗ 
+        ∀ e_t' σ_t',
+          ⌜prim_step P_t (e_t, σ_t) (e_t', σ_t')⌝ ==∗
+            ∃ e_s' σ_s', ⌜rtc (prim_step P_s) (e_s, σ_s) (e_s', σ_s')⌝ ∗
+              state_interp P_t σ_t' P_s σ_s' ∗ e_t' ⪯ e_s' {{ Φ }}) -∗
+      e_t ⪯ e_s {{ Φ }}.
     Proof.
       iIntros "H". rewrite (sim_unfold Φ e_t e_s). iIntros (????) "[Hstate %]".
       iMod ("H" with "Hstate") as "[Hred H]". iModIntro. iRight; iLeft.
@@ -624,7 +651,7 @@ Section fix_lang.
   Section no_stuttering.
     (** Simpler relation without stuttering using just a greatest fp. *)
 
-    Definition step_nostutter (Φ : val Λ → val Λ → PROP) (greatest_rec : exprO * exprO → PROP) : exprO * exprO → PROP:=
+    Definition step_nostutter Φ (greatest_rec : exprO * exprO → PROP) : exprO * exprO → PROP:=
       λ '(e_s, e_t), (∀ P_t σ_t P_s σ_s, state_interp P_t σ_t P_s σ_s ∗ ⌜¬ reach_stuck P_s e_s σ_s⌝ -∗ |==>
         (* value case *)
         (∃ v_t v_s σ_s', ⌜to_val e_t = Some v_t⌝ ∗ ⌜rtc (prim_step P_s) (e_s, σ_s) (of_val v_s, σ_s')⌝ ∗
@@ -641,7 +668,7 @@ Section fix_lang.
           (∀ v_t v_s, val_rel v_t v_s -∗ greatest_rec (fill K_s (of_val v_s), fill K_t (of_val v_t))))
       )%I.
 
-    Definition sim_nostutter_def (Φ : val Λ → val Λ → PROP) :=
+    Definition sim_nostutter_def Φ :=
       bi_greatest_fixpoint (step_nostutter Φ).
 
     Instance step_nostutter_proper:
@@ -650,7 +677,7 @@ Section fix_lang.
         ==> (≡) ==> (≡)) (step_nostutter).
     Proof. solve_proper. Qed.
 
-    Instance step_nostutter_mono (Φ : val Λ → val Λ → PROP):
+    Instance step_nostutter_mono Φ:
       BiMonoPred (step_nostutter Φ).
     Proof.
       constructor.
@@ -667,17 +694,18 @@ Section fix_lang.
           iExists (f), (K_t), (v_t), (K_s), (v_s), (σ_s'). iFrame.
           iIntros (? ?) "H1". iApply "H". by iApply "H5".
       - intros g Hne n e1 e2 Heq.
-        apply discrete_iff in Heq as ->. reflexivity. apply _.
+        apply (discrete_iff _ _) in Heq as ->. done.
     Qed.
 
     Lemma sim_nostutter_def_unfold Φ e_s e_t:
       sim_nostutter_def Φ (e_s, e_t) ⊣⊢ step_nostutter Φ (sim_nostutter_def Φ) (e_s, e_t).
     Proof. by rewrite /sim_nostutter_def greatest_fixpoint_unfold. Qed.
 
-    Definition sim_nostutter_aux : seal (λ e_t e_s Φ, @sim_nostutter_def Φ (e_s, e_t)). by eexists. Qed.
-    Instance sim_nostutter : Sim s. exact ((sim_nostutter_aux).(unseal)). Defined.
-    Definition sim_nostutter_eq : sim_nostutter = λ e_t e_s Φ, @sim_nostutter_def Φ (e_s, e_t).
-      by rewrite <- (sim_nostutter_aux).(seal_eq). Defined.
+    Definition sim_nostutter_aux : seal (λ e_t e_s Φ, @sim_nostutter_def Φ (e_s, e_t)).
+    Proof. by eexists. Qed.
+    Instance sim_nostutter : Sim s := sim_nostutter_aux.(unseal).
+    Lemma sim_nostutter_eq : sim (Sim:=sim_nostutter) = λ e_t e_s Φ, @sim_nostutter_def Φ (e_s, e_t).
+    Proof. by rewrite <-sim_nostutter_aux.(seal_eq). Qed.
 
     Lemma sim_nostutter_unfold e_t e_s Φ:
       sim (Sim:=sim_nostutter) e_t e_s Φ ⊣⊢
@@ -689,29 +717,31 @@ Section fix_lang.
         ∨ (* step case *)
         (⌜reducible P_t e_t σ_t⌝ ∗ ∀ e_t' σ_t', ⌜prim_step P_t (e_t, σ_t) (e_t', σ_t')⌝ -∗ |==>
           ∃ e_s' σ_s', ⌜tc (prim_step P_s) (e_s, σ_s) (e_s', σ_s')⌝ ∗ state_interp P_t σ_t' P_s σ_s' ∗
-          sim (Sim:=sim_nostutter) e_t' e_s' Φ)
+          sim e_t' e_s' Φ)
 
         ∨ (* call case *)
         (∃ f K_t v_t K_s v_s σ_s', ⌜e_t = fill K_t (of_call f v_t)⌝ ∗
           ⌜rtc (prim_step P_s) (e_s, σ_s) (fill K_s (of_call f v_s), σ_s')⌝ ∗
           val_rel v_t v_s ∗ state_interp P_t σ_t P_s σ_s' ∗
-          sim_ectx (sim:=sim_nostutter) K_t K_s Φ)
+          sim_ectx K_t K_s Φ)
       )%I.
     Proof.
-      by rewrite /sim_ectx /sim !sim_nostutter_eq /uncurry sim_nostutter_def_unfold /step_nostutter.
+      by rewrite /sim_ectx !sim_nostutter_eq /uncurry sim_nostutter_def_unfold /step_nostutter.
     Qed.
 
     Lemma sim_nostutter_coind Φ (Ψ : exprO → exprO → PROP):
       Proper ((≡) ==> (≡) ==> (≡)) Ψ →
-      ⊢ (□ ∀ e_t e_s, Ψ e_t e_s -∗ step_nostutter Φ (λ '(e_s', e_t'), Ψ e_t' e_s') (e_s, e_t))
-        → (∀ e_t e_s, Ψ e_t e_s -∗ e_t ⪯ e_s {{Φ}}).
+      (□ ∀ e_t e_s, Ψ e_t e_s -∗ step_nostutter Φ (λ '(e_s', e_t'), Ψ e_t' e_s') (e_s, e_t)) -∗
+      (∀ e_t e_s, Ψ e_t e_s -∗ e_t ⪯ e_s {{ Φ }}).
     Proof.
       iIntros (Hp) "#IH". iIntros (e_t e_s) "H".
-      rewrite /sim sim_nostutter_eq /sim_nostutter_def.
+      rewrite sim_nostutter_eq /sim_nostutter_def.
       set (Ψ_curry := (λ '(e_t, e_s), Ψ e_s e_t)).
       assert (NonExpansive Ψ_curry) as Hne.
       { intros ? [e1 e2] [e1' e2'] [H1 H2]. rewrite /Ψ_curry. cbn in H1, H2.
-        apply equiv_dist, Hp. now apply discrete_iff in H1. now apply discrete_iff in H2.
+        apply equiv_dist, Hp.
+        - by apply (discrete_iff _ _) in H1.
+        - by apply (discrete_iff _ _) in H2.
       }
 
       iApply (greatest_fixpoint_coind (step_nostutter Φ) Ψ_curry with "[]").
@@ -720,26 +750,30 @@ Section fix_lang.
     Qed.
 
     Instance sim_nostutter_proper :
-      Proper (eq ==> eq ==> (pointwise_relation (val Λ) (pointwise_relation (val Λ) (≡))) ==> (≡)) sim.
+      Proper (eq ==> eq ==>
+        (pointwise_relation (val Λ) (pointwise_relation (val Λ) (≡))) ==> (≡)) sim.
     Proof.
       intros e e' -> e1 e1' -> p1 p2 Heq2.
-      rewrite /sim !sim_nostutter_eq. apply greatest_fixpoint_proper; solve_proper.
+      rewrite !sim_nostutter_eq. apply greatest_fixpoint_proper; solve_proper.
     Qed.
 
-    Lemma sim_nostutter_value Φ v_t v_s:
-      ⊢ Φ v_t v_s -∗ (of_val v_t) ⪯ (of_val v_s) {{Φ}}.
+    Lemma sim_nostutter_value Φ v_t v_s :
+      ⊢ Φ v_t v_s -∗ (of_val v_t) ⪯ (of_val v_s) {{ Φ }}.
     Proof.
       iIntros "Hv". rewrite sim_nostutter_unfold. iIntros (????) "[Hstate Hreach]".
       iModIntro. iLeft. iExists (v_t), (v_s), (σ_s). iFrame.
-      iSplitL. by rewrite to_of_val. eauto.
+      iSplitL; first by rewrite to_of_val. eauto.
     Qed.
 
-    Lemma sim_nostutter_call P_t P_s v_t v_s K_t K_s f Φ:
+    Lemma sim_nostutter_call P_t P_s v_t v_s K_t K_s f Φ :
       P_t !! f = Some K_t →
       P_s !! f = Some K_s →
-      ⊢ progs_are P_t P_s ∗ val_rel v_t v_s ∗ sim_ectx K_t K_s Φ -∗ (of_call f v_t) ⪯ (of_call f v_s) {{Φ}}.
+      progs_are P_t P_s -∗
+      val_rel v_t v_s -∗
+      sim_ectx K_t K_s Φ -∗
+      (of_call f v_t) ⪯ (of_call f v_s) {{ Φ }}.
     Proof.
-      intros Htgt Hsrc. iIntros "(#Prog & Val & Sim)".
+      intros Htgt Hsrc. iIntros "#Prog Val Sim".
       rewrite sim_nostutter_unfold. iIntros (P_t' σ_t P_s' σ_s) "[SI %]".
       iModIntro. iRight. iLeft.
       rewrite /progs_are; iDestruct ("Prog" with "SI") as "[% %]"; subst P_t' P_s'; iClear "Prog".
@@ -754,21 +788,21 @@ Section fix_lang.
         + rewrite fill_empty; assert (K_t' = K_t) as -> by naive_solver. iApply ("Sim" with "Val").
     Qed.
 
-    Lemma bupd_sim_nostutter Φ e_t e_s:
-      ⊢ (|==> e_t ⪯ e_s {{Φ}}) -∗ e_t ⪯ e_s {{Φ}}.
+    Lemma bupd_sim_nostutter Φ e_t e_s :
+      ⊢ (|==> e_t ⪯ e_s {{Φ}}) -∗ e_t ⪯ e_s {{ Φ }}.
     Proof.
       iIntros "Hv". rewrite sim_nostutter_unfold. iIntros (????) "H". iMod "Hv". iApply ("Hv" with "H").
     Qed.
 
-    Lemma sim_nostutter_mono Φ Φ':
+    Lemma sim_nostutter_mono Φ Φ' :
       ⊢ (∀ v_t v_s, Φ v_t v_s -∗ Φ' v_t v_s)
-         -∗ ∀ e_s e_t : exprO, e_t ⪯ e_s {{Φ}} -∗ e_t ⪯ e_s {{Φ'}}.
+         -∗ ∀ e_s e_t : exprO, e_t ⪯ e_s {{ Φ }} -∗ e_t ⪯ e_s {{ Φ' }}.
     Proof.
       iIntros "Hmon".
       iIntros (e_s e_t) "H".
-      iApply (sim_nostutter_coind Φ' (λ e_t e_s, e_t ⪯ e_s {{Φ}} ∗ (∀ v_t v_s : val Λ, Φ v_t v_s -∗ Φ' v_t v_s))%I); last by iFrame.
+      iApply (sim_nostutter_coind Φ' (λ e_t e_s, e_t ⪯ e_s {{ Φ }} ∗ (∀ v_t v_s : val Λ, Φ v_t v_s -∗ Φ' v_t v_s))%I); last by iFrame.
       iModIntro. clear e_t e_s. iIntros (e_t e_s) "[H Hpost]".
-      rewrite /sim sim_nostutter_eq sim_nostutter_def_unfold.
+      rewrite sim_nostutter_eq sim_nostutter_def_unfold.
       rewrite /step_nostutter.
       iIntros (????) "Hs". iSpecialize ("H" with "Hs"). iMod "H". iModIntro.
       iDestruct "H" as "[Hval | [Hred | Hcall]]".
@@ -812,11 +846,12 @@ Section fix_lang.
     Proof.
       (* unfold Hpost to examine the result and combine the two simulation proofs *)
       iIntros (H0 H Hnreach) "Hpost Hstate".
-      rewrite {1}/sim {1}sim_nostutter_eq {1}sim_nostutter_def_unfold.
+      rewrite {1}sim_nostutter_eq {1}sim_nostutter_def_unfold.
       rewrite {1}/step_nostutter.
       iMod ("Hpost" with "[Hstate]") as "Hpost".
-      { iFrame. iPureIntro. intros Hstuck. eapply Hnreach, prim_step_rtc_reach_stuck.
-        by apply fill_prim_step_rtc. assumption. }
+      { iFrame. iPureIntro. intros Hstuck.
+        eapply Hnreach, prim_step_rtc_reach_stuck; last done.
+        by apply fill_prim_step_rtc. }
       iModIntro.
       iDestruct "Hpost" as "[Hv | [Hstep | Hcall]]".
       + iLeft. iDestruct "Hv" as (v_t' v_s' σ_s'') "(% & % & Hstate & Hpost)".
@@ -828,27 +863,26 @@ Section fix_lang.
         iIntros (e_t' σ_t') "%". iMod ("Hstep" with "[]") as "Hstep".
         { iPureIntro. by rewrite (of_to_val _ _ H). }
         iDestruct "Hstep" as (e_s' σ_s'') "(%&Hstate& Hrec)".
-        iExists e_s', σ_s''. iFrame. iSplitL "".
+        iExists e_s', σ_s''. iFrame. iSplitR.
         { iPureIntro. eapply tc_rtc_l; by eauto using fill_prim_step_rtc. }
         cbn. iExists e_t', e_s', empty_ectx, empty_ectx. rewrite !fill_empty.
-        do 2 (iSplitL ""; first auto).
-        iApply sim_nostutter_mono. 2: { rewrite /sim sim_nostutter_eq. iApply "Hrec". }
+        do 2 (iSplitR; first auto).
+        iApply sim_nostutter_mono. 2: { rewrite sim_nostutter_eq. iApply "Hrec". }
         iIntros (??) "H". rewrite !fill_empty.
         by iApply sim_nostutter_value.
       + iDestruct "Hcall" as (f K_t' v_t' K_s' v_s' σ_s'') "(%&%&Hvrel&Hstate&Hcall)".
         (* CA on the reduction of fill K_s v_s to fill K_s' (f v_s') to see if we need to take a step or do the call *)
         iRight; iRight.
         iExists f, K_t', v_t', K_s', v_s', σ_s''. iFrame.
-        iSplitL "". { iPureIntro. by rewrite -H1 (of_to_val _ _ H). }
-        iSplitL "". { iPureIntro. etrans; by eauto using fill_prim_step_rtc. }
+        iSplitR. { iPureIntro. by rewrite -H1 (of_to_val _ _ H). }
+        iSplitR. { iPureIntro. etrans; by eauto using fill_prim_step_rtc. }
         iIntros (v_t'' v_s'') "Hvrel". cbn.
         iExists (fill K_t' (of_val v_t'')), (fill K_s' (of_val v_s'')), empty_ectx, empty_ectx.
-        rewrite !fill_empty. do 2 (iSplitL ""; first auto).
+        rewrite !fill_empty. do 2 (iSplitR; first auto).
         iApply sim_nostutter_mono; first last.
-        { rewrite /sim sim_nostutter_eq. by iApply "Hcall". }
+        { rewrite sim_nostutter_eq. by iApply "Hcall". }
         iIntros (??) "H". rewrite !fill_empty. by iApply sim_nostutter_value.
     Qed.
-
 
     Lemma sim_nostutter_bind e_t e_s K_t K_s Φ:
       ⊢ e_t ⪯ e_s {{λ v_t v_s : val Λ, fill K_t (of_val v_t) ⪯ fill K_s (of_val v_s) {{Φ}} }}
@@ -860,7 +894,7 @@ Section fix_lang.
       iModIntro. clear e_t e_s K_t K_s.
       iIntros (e_t' e_s') "IH".
       iDestruct "IH" as (e_t e_s K_t K_s) "[-> [-> H]]".
-      rewrite {1}/sim {1}sim_nostutter_eq {1}sim_nostutter_def_unfold.
+      rewrite {1}sim_nostutter_eq {1}sim_nostutter_def_unfold.
       rewrite /step_nostutter.
 
       iIntros (????) "[Hs %]". rename H into Hnreach.
@@ -871,31 +905,29 @@ Section fix_lang.
         by iApply (sim_bind_val_nostutter with "[Hpost] [Hstate]").
       - (* simply thread through everything *)
         iModIntro. iRight; iLeft. iDestruct "Hstep" as "[% Hstep]".
-        iSplitL "". { iPureIntro. by apply fill_reducible. }
+        iSplitR. { iPureIntro. by apply fill_reducible. }
         iIntros (e_t' σ_t') "%".
         destruct (fill_reducible_prim_step _ _ _ _ _ _ H H0) as (e_t'' & -> & H1).
         iMod ("Hstep" with "[]") as "Hstep". { iPureIntro. apply H1. }
         iModIntro.
         iDestruct "Hstep" as (e_s' σ_s') "(% & Hstate & Hrec)".
-        iExists (fill K_s e_s'), σ_s'. iFrame. iSplitL "".
+        iExists (fill K_s e_s'), σ_s'. iFrame. iSplitR.
         { iPureIntro. by apply fill_prim_step_tc. }
         cbn. iExists e_t'', e_s', K_t, K_s.
-        do 2 (iSplitL ""; first auto).
-        rewrite /sim sim_nostutter_eq. iApply "Hrec".
+        do 2 (iSplitR; first auto).
+        rewrite sim_nostutter_eq. iApply "Hrec".
       - (* simply thread through everything *)
         iModIntro. iRight; iRight.
         iDestruct "Hcall" as (f K_t' v_t K_s' v_s σ_s') "(-> & % & Hval & Hstate & Hrec)".
         iExists f, (comp_ectx K_t K_t'), v_t, (comp_ectx K_s K_s'), v_s, σ_s'.
-        iSplitL "". by rewrite fill_comp.
-        iSplitL "". { iPureIntro. rewrite -fill_comp. by apply fill_prim_step_rtc. }
+        iSplitR; first by rewrite fill_comp.
+        iSplitR. { iPureIntro. rewrite -fill_comp. by apply fill_prim_step_rtc. }
         iFrame.
         iIntros (v_t' v_s') "Hv". iSpecialize ("Hrec" with "Hv"). cbn.
         iExists (fill K_t' (of_val v_t')), (fill K_s' (of_val v_s')), K_t, K_s.
-        iSplitL "". by rewrite -fill_comp. iSplitL "". by rewrite -fill_comp.
-        rewrite /sim sim_nostutter_eq. iApply "Hrec".
+        iSplitR; first by rewrite -fill_comp. iSplitR; first by rewrite -fill_comp.
+        rewrite sim_nostutter_eq. iApply "Hrec".
     Qed.
-
-
 
   End no_stuttering.
 End fix_lang.
