theories/simulation/stutter_adequacy.v
@@ -12,17 +12,18 @@ From simuliris.simulation Require Import relations language slsls.
 *)
 
 Section fix_lang.
-  Context {PROP : bi}.
+  Context {PROP : bi} `{!BiBUpd PROP, !BiAffine PROP, !BiPureForall PROP}.
 
   Context {Λ : language}.
-  Context {s : simul_lang PROP Λ}.
-  Context {PROP_bupd : BiBUpd PROP}.
-  Context {PROP_affine : BiAffine PROP}.
+  Context {s : SimulLang PROP Λ}.
 
   Implicit Types
-    (e_s e_t e: exprO (Λ := Λ))
-    (P_s P_t P: prog Λ)
-    (σ_s σ_t σ : state Λ).
+    (e_s e_t e : expr Λ)
+    (P_s P_t P : prog Λ)
+    (σ_s σ_t σ : state Λ)
+    (Φ Ψ : val Λ → val Λ → PROP).
+
+  Local Existing Instance sim_stutter.
 
 Section global.
 
@@ -147,10 +148,10 @@ End global.
 Section local_to_global.
 
   Definition local_rel P_t P_s : PROP :=
-    (□ ∀ f K_s, ⌜P_s !! f = Some K_s⌝ → ∃ K_t, ⌜P_t !! f = Some K_t⌝ ∗ sim_ectx (sim:=sim_stutter) K_t K_s val_rel)%I.
+    (□ ∀ f K_s, ⌜P_s !! f = Some K_s⌝ → ∃ K_t, ⌜P_t !! f = Some K_t⌝ ∗ sim_ectx K_t K_s val_rel)%I.
   Typeclasses Opaque local_rel.
 
-  Global Instance local_rel_persistent P_s P_t: Persistent (local_rel P_s P_t).
+  Global Instance local_rel_persistent P_s P_t : Persistent (local_rel P_s P_t).
   Proof. rewrite /local_rel; apply _. Qed.
 
   Lemma gsim_coind Φ (Ψ : exprO → exprO → PROP):
@@ -180,7 +181,7 @@ Section local_to_global.
     iIntros "#Hloc #Hprog Hsim".
     iApply (gsim_coind val_rel (λ e_t e_s, sim (Sim:=sim_stutter) e_t e_s val_rel) with "[] Hsim"); clear e_t e_s.
     iModIntro. iIntros (e_t e_s).
-    rewrite /greatest_step {1}/sim sim_eq sim_def_unfold /slsls.greatest_step.
+    rewrite /greatest_step sim_eq sim_def_unfold /slsls.greatest_step.
     iRevert (e_t). iApply sim_ind. iModIntro. iIntros (e_t).
     rewrite /slsls.least_step least_def_unfold /least_step.
     iIntros "Hsim" (P_t' σ_t P_s' σ_s) "[Hstate %]".
@@ -204,10 +205,10 @@ Section local_to_global.
       iFrame. iSplit.
       + iPureIntro. eapply tc_rtc_l; first by eauto.
         constructor. by apply fill_prim_step, head_prim_step, call_head_step_intro.
-      + rewrite /uncurry. rewrite -!sim_eq. iPoseProof (sim_bind _ _ K_t K_s val_rel with "[Hval Hcont]") as "HP"; last first.
-        { rewrite /sim sim_eq; iApply "HP". }
+      + rewrite /uncurry. iPoseProof (sim_bind _ _ K_t K_s val_rel with "[Hval Hcont]") as "HP"; last first.
+        { rewrite sim_eq; iApply "HP". }
         iApply (sim_mono with "[Hcont] [Hval]").
-        * rewrite /sim sim_eq. iExact "Hcont".
+        * rewrite sim_eq. iExact "Hcont".
         * rewrite /local_rel; iDestruct ("Hloc" $! _ _ Hdef_s) as (K_f_t') "[% Hcont]".
           assert (K_f_t' = K_f_t) as -> by naive_solver.
           iSpecialize ("Hcont" with "Hval").
@@ -224,7 +225,7 @@ Section meta_level_simulation.
 
   Context {PROP : bi}.
   Context {Λ : language}.
-  Context {s : simul_lang PROP Λ}.
+  Context {s : SimulLang PROP Λ}.
   Context {PROP_bupd : BiBUpd PROP}.
   Context {PROP_affine : BiAffine PROP}.
   Context {sat: PROP → Prop} {Sat: Satisfiable sat}.
@@ -360,7 +361,7 @@ Section simulation_behaviorally_related.
 
   Context {PROP : bi}.
   Context {Λ : language}.
-  Context {s : simul_lang PROP Λ}.
+  Context {s : SimulLang PROP Λ}.
   Context {PROP_bupd : BiBUpd PROP}.
   Context {PROP_affine : BiAffine PROP}.
   Context {sat: PROP → Prop} {Sat: Satisfiable sat}.
@@ -442,11 +443,9 @@ End simulation_behaviorally_related.
 
 
 Section adequacy_statement.
-  Context {PROP : bi}.
+  Context {PROP : bi} `{!BiBUpd PROP, !BiAffine PROP, !BiPureForall PROP}.
   Context {Λ : language}.
-  Context {s : simul_lang PROP Λ}.
-  Context {PROP_bupd : BiBUpd PROP}.
-  Context {PROP_affine : BiAffine PROP}.
+  Context {s : SimulLang PROP Λ}.
   Context {sat: PROP → Prop} {Sat: Satisfiable sat}.
   Arguments sat _%I.
 
@@ -471,7 +470,7 @@ Section adequacy_statement.
       progs_are P_t P_s ∗
       val_rel u u) →
     (* post *)
-    (∀ v_t v_s σ_t σ_s, sat (state_interp P_t σ_t P_s σ_s ∗ val_rel (simul_lang := s) v_t v_s) → O v_t v_s) →
+    (∀ v_t v_s σ_t σ_s, sat (state_interp P_t σ_t P_s σ_s ∗ val_rel (SimulLang := s) v_t v_s) → O v_t v_s) →
     B P_t P_s.
   Proof.
     intros Hpre Hpost σ_t σ_s [HI Hstuck].
@@ -496,11 +495,9 @@ End adequacy_statement.
 
 Section adequacy_statement_alt.
 
-  Context {PROP : bi}.
+  Context {PROP : bi} `{!BiBUpd PROP, !BiAffine PROP, !BiPureForall PROP}.
   Context {Λ : language}.
-  Context {s : simul_lang PROP Λ}.
-  Context {PROP_bupd : BiBUpd PROP}.
-  Context {PROP_affine : BiAffine PROP}.
+  Context {s : SimulLang PROP Λ}.
   Context {sat: PROP → Prop} {Sat: Satisfiable sat}.
   Arguments sat _%I.
 
@@ -513,13 +510,13 @@ Section adequacy_statement_alt.
       (∀ σ_t σ_s, ⌜I σ_t σ_s⌝ -∗ state_interp P_t σ_t P_s σ_s) ∗
       progs_are P_t P_s ∗
       val_rel u u ∗
-      ∀ v_s v_t, val_rel (simul_lang := s) v_t v_s -∗ ⌜O v_t v_s⌝) →
+      ∀ v_s v_t, val_rel (SimulLang := s) v_t v_s -∗ ⌜O v_t v_s⌝) →
     B I O main u P_t P_s.
   Proof.
     intros Hsat. eapply sat_frame_intro in Hsat; last first.
     { iIntros "(H1 & H2 & H3 & H4 & F)". iSplitL "F"; first iExact "F".
       iCombine "H1 H2 H3 H4" as "H". iExact "H". }
-    eapply (@adequacy PROP _ _ _ _ (sat_frame _) _); first apply Hsat.
+    eapply (@adequacy PROP _ _ _ _ _ (sat_frame _) _); first apply Hsat.
     intros v_t v_s σ_t σ_s Hsat_post. eapply sat_elim, sat_mono, Hsat_post.
     iIntros "(H & _ & Hval)". by iApply "H".
   Qed.
